lib/coq/go.sh
@@ -1,6 +1,5 @@
 opam switch 4.09.1
 eval $(opam env)
 PATH=~/versions/coq-8.12/coq/bin:$PATH
-make _CoqProject
 make
 
